Add unit tests for consistency predicate

test/test_predicate_provability.dfy
@@ -1,5 +1,88 @@
 include "../dafny/ver/L1/theorems.dfy"
 
+/*
+// mutant 1: makes all provability tests fail
+predicate consistency(t: Trace)
+    {
+        forall i,n1,n2 
+        |
+                    && n1 in t(i).nodes.Keys
+                    && n2 in t(i).nodes.Keys
+                    // && isHonest(t(i),n1)
+                    // && isHonest(t(i),n2)
+                ::
+                consistentBlockchains(t(i).nodes[n1].blockchain, t(i).nodes[n2].blockchain)
+    } 
+*/
+
+/*
+// mutant 2: makes two provability tests fail
+predicate consistentBlockchains(bc1:Blockchain, bc2:Blockchain)
+    {
+        || bc1 <= bc2
+        || bc2 <= bc1
+            // var rbc1 := fromBlockchainToRawBlockchain(bc1);
+            // var rbc2 := fromBlockchainToRawBlockchain(bc2);
+            // || rbc1 <= rbc2
+            // || rbc2 <= rbc1 
+    }     
+*/
+
+/*
+// mutant 3: makes one correctness test fail
+predicate consistentBlockchains(bc1:Blockchain, bc2:Blockchain)
+    {
+        forall i:nat | 0 < i < |bc1| && i < |bc2| ::fromBlockToRawBlock(bc1[i]) == fromBlockToRawBlock(bc2[i])
+            // var rbc1 := fromBlockchainToRawBlockchain(bc1);
+            // var rbc2 := fromBlockchainToRawBlockchain(bc2);
+            // || rbc1 <= rbc2
+            // || rbc2 <= rbc1
+    } 
+
+*/
+
+/*
+// mutant 4: wrong variable substitution (n2 -> n1)
+predicate consistency(t: Trace)
+    {
+        forall i,n1,n2 |
+                    // && n1 in t(i).nodes.Keys
+                    // && n2 in t(i).nodes.Keys
+                    && isHonest(t(i),n1)
+                    && isHonest(t(i),n2)
+                ::
+                consistentBlockchains(t(i).nodes[n1].blockchain, t(i).nodes[n1].blockchain)
+    }  
+*/
+
+/*
+// mutant 5: || -> &&
+predicate consistentBlockchains(bc1:Blockchain, bc2:Blockchain)
+    {
+        // || bc1 <= bc2
+        // || bc2 <= bc1
+        // forall i:nat | 0 < i < |bc1| && i < |bc2| ::fromBlockToRawBlock(bc1[i]) == fromBlockToRawBlock(bc2[i])
+            var rbc1 := fromBlockchainToRawBlockchain(bc1);
+            var rbc2 := fromBlockchainToRawBlockchain(bc2);
+            && rbc1 <= rbc2
+            && rbc2 <= rbc1
+    }     
+
+*/
+
+/* 
+// mutant 6: <= -> <
+predicate consistentBlockchains(bc1:Blockchain, bc2:Blockchain)
+    {
+        // || bc1 <= bc2
+        // || bc2 <= bc1
+        // forall i:nat | 0 < i < |bc1| && i < |bc2| ::fromBlockToRawBlock(bc1[i]) == fromBlockToRawBlock(bc2[i])
+            var rbc1 := fromBlockchainToRawBlockchain(bc1);
+            var rbc2 := fromBlockchainToRawBlockchain(bc2);
+            || rbc1 < rbc2
+            || rbc2 < rbc1
+    }     
+*/
 module test_consistency_provability {
     import opened L1_SpecTypes
     import opened L1_SpecNetwork
@@ -36,9 +119,8 @@ module test_consistency_provability {
     lemma test_consistency_provability_3(t:Trace)
         // one empty blockchain
         requires forall i, j :: t(i) == t(j)
-        requires t(0).nodes.Keys == {0,1,2}
-        requires t(0).adversary.byz == {}
-        requires t(0).nodes[1].blockchain <= t(0).nodes[0].blockchain || t(0).nodes[0].blockchain <= t(0).nodes[1].blockchain
+        requires t(0).nodes.Keys - t(0).adversary.byz == {0,1,2}
+        requires fromBlockchainToRawBlockchain(t(0).nodes[1].blockchain) <= fromBlockchainToRawBlockchain(t(0).nodes[0].blockchain) || fromBlockchainToRawBlockchain(t(0).nodes[0].blockchain) <= fromBlockchainToRawBlockchain(t(0).nodes[1].blockchain)
         requires t(0).nodes[2].blockchain == []
         ensures consistency(t)
     {}
@@ -46,11 +128,10 @@ module test_consistency_provability {
     lemma test_consistency_provability_4(t:Trace)
         // one empty blockchain
         requires forall i, j :: t(i) == t(j)
-        requires t(0).nodes.Keys == {0,1,2}
-        requires t(0).adversary.byz == {}
+        requires t(0).nodes.Keys - t(0).adversary.byz == {0,1,2}
         requires |t(0).nodes[0].blockchain| == 1
         requires |t(0).nodes[1].blockchain| > 1
-        requires t(0).nodes[1].blockchain[0] == t(0).nodes[0].blockchain[0]
+        requires fromBlockToRawBlock(t(0).nodes[1].blockchain[0]) == fromBlockToRawBlock(t(0).nodes[0].blockchain[0])
         requires t(0).nodes[2].blockchain == []
         ensures consistency(t)
     {}
@@ -58,18 +139,22 @@ module test_consistency_provability {
     lemma test_consistency_provability_5(t:Trace)
         // one empty blockchain
         requires forall i, j :: t(i) == t(j)
-        requires t(0).nodes.Keys == {0,1,2}
-        requires t(0).adversary.byz == {}
-        requires t(0).nodes[1].blockchain == t(0).nodes[0].blockchain
+        requires t(0).nodes.Keys - t(0).adversary.byz == {0,1,2}
+        requires fromBlockchainToRawBlockchain(t(0).nodes[1].blockchain) == fromBlockchainToRawBlockchain(t(0).nodes[0].blockchain)
         requires t(0).nodes[2].blockchain == []
         ensures consistency(t)
-    {}
+    {
+        forall i:nat | i < |t(0).nodes[1].blockchain| 
+            ensures fromBlockToRawBlock(t(0).nodes[1].blockchain[i]) == fromBlockToRawBlock(t(0).nodes[0].blockchain[i]) 
+        {
+            assert fromBlockchainToRawBlockchain(t(0).nodes[1].blockchain)[i] == fromBlockchainToRawBlockchain(t(0).nodes[0].blockchain)[i];
+        }
+    }
 
     lemma test_consistency_provability_6(t:Trace)
         // one empty blockchain
         requires forall i, j :: t(i) == t(j)
-        requires t(0).nodes.Keys == {0,1,2}
-        requires t(0).adversary.byz == {}
+        requires t(0).nodes.Keys - t(0).adversary.byz == {0,1,2}
         requires |t(0).nodes[0].blockchain| == 3
         requires |t(0).nodes[1].blockchain| >= 3
         requires t(0).nodes[1].blockchain[0] == t(0).nodes[0].blockchain[0]
@@ -81,16 +166,14 @@ module test_consistency_provability {
 
     lemma test_consistency_provability_7(t:Trace)
         requires forall i, j :: t(i) == t(j)
-        requires t(0).nodes.Keys == {0,1,2}
-        requires t(0).adversary.byz == {}
+        requires t(0).nodes.Keys - t(0).adversary.byz == {0,1,2}
         requires t(0).nodes[0].blockchain == t(0).nodes[1].blockchain == t(0).nodes[2].blockchain
         ensures consistency(t)
     {}
 
     lemma test_consistency_provability_8(t:Trace)
         requires forall i, j :: t(i) == t(j)
-        requires t(0).nodes.Keys == {0,1,2}
-        requires t(0).adversary.byz == {}
+        requires t(0).nodes.Keys - t(0).adversary.byz == {0,1,2}
         requires |t(0).nodes[0].blockchain| == 1
         requires |t(0).nodes[1].blockchain| > 1
         requires t(0).nodes[1].blockchain[0] == t(0).nodes[0].blockchain[0]
@@ -100,8 +183,17 @@ module test_consistency_provability {
 
     lemma test_consistency_provability_9(t:Trace)
         requires forall i, j :: t(i) == t(j)
-        requires t(0).nodes.Keys == {0,1,2}
-        requires t(0).adversary.byz == {}
+        requires t(0).nodes.Keys - t(0).adversary.byz == {0,1,2}
+        requires |t(0).nodes[0].blockchain| > 1
+        requires |t(0).nodes[1].blockchain| == 1
+        requires t(0).nodes[1].blockchain[0] == t(0).nodes[0].blockchain[0]
+        requires t(0).nodes[1].blockchain == t(0).nodes[2].blockchain
+        ensures consistency(t)
+    {}
+
+    lemma test_consistency_provability_10(t:Trace)
+        requires forall i, j :: t(i) == t(j)
+        requires t(0).nodes.Keys - t(0).adversary.byz == {0,1,2}
         requires |t(0).nodes[0].blockchain| == 1
         requires |t(0).nodes[1].blockchain| == 3
         requires t(0).nodes[1].blockchain[0] == t(0).nodes[0].blockchain[0]
@@ -111,4 +203,42 @@ module test_consistency_provability {
         requires t(0).nodes[1].blockchain[2] == t(0).nodes[2].blockchain[2]
         ensures consistency(t)
     {}
+
+    lemma test_consistency_provability_non_const_t(t:Trace)
+        requires forall i | i > 1 :: t(i) == t(1)
+        requires t(1).nodes.Keys - t(1).adversary.byz == {0,1,2}
+        requires t(1).nodes[0].blockchain == []
+        requires t(1).nodes[1].blockchain == []
+        requires t(0).nodes.Keys - t(0).adversary.byz == {0,1,2}
+        requires t(0).nodes[1].blockchain <= t(0).nodes[0].blockchain || t(0).nodes[0].blockchain <= t(0).nodes[1].blockchain
+        requires t(0).nodes[2].blockchain == []
+        ensures consistency(t)
+    {}
+
+    lemma test_consistency_provability_no_node(t:Trace)
+        requires forall i, j :: t(i) == t(j)
+        requires t(0).nodes.Keys - t(0).adversary.byz == {}
+        ensures consistency(t)
+    {}
+
+    lemma test_consistency_provability_one_node(t:Trace)
+        requires forall i, j :: t(i) == t(j)
+        requires t(0).nodes.Keys - t(0).adversary.byz == {0}
+        ensures consistency(t)
+    {}
+
+    lemma test_consistency_provability_one_node'(t:Trace)
+        requires forall i, j :: t(i) == t(j)
+        requires t(0).nodes.Keys - t(0).adversary.byz == {5}
+        ensures consistency(t)
+    {}
+
+    lemma test_consistency_provability_two_nodes(t:Trace)
+        requires forall i, j :: t(i) == t(j)
+        requires t(0).nodes.Keys - t(0).adversary.byz == {0,1}
+        requires t(0).nodes[1].blockchain <= t(0).nodes[0].blockchain || t(0).nodes[0].blockchain <= t(0).nodes[1].blockchain
+        ensures consistency(t)
+    {}
+
+
 }
