dafny/ver/L1/theorems_defs.dfy
@@ -9,6 +9,9 @@ module L1_TheoremsDefs {
 
     predicate consistentBlockchains(bc1:Blockchain, bc2:Blockchain)
     {
+        // || bc1 <= bc2
+        // || bc2 <= bc1
+        // forall i:nat | 0 < i < |bc1| && i < |bc2| ::fromBlockToRawBlock(bc1[i]) == fromBlockToRawBlock(bc2[i])
             var rbc1 := fromBlockchainToRawBlockchain(bc1);
             var rbc2 := fromBlockchainToRawBlockchain(bc2);
             || rbc1 <= rbc2
